App/Lib/Iterator/Spec.v
@@ -9,7 +9,7 @@ Section Specs.
 Open Scope oo_scope.
 
 Variable step : step_relation.
-Variable wf : tm -> state -> Prop.
+Variable wf : term -> state -> Prop.
 
 Notation "t1 '/' st1 '==>' t2 '/' st2" := (step (Cexec_state t1 st1) (Cexec_state t2 st2))
   (at level 40, st1 at level 39, t2 at level 39, format "'[' t1 / st1 '==>' t2 / st2 ']'").
