He4/Language/Stack.v
@@ -4,7 +4,7 @@ Require Import He4.Lists.List.
 
 (** * Types *)
 
-Definition stack_frame : Type := list tm.
+Definition stack_frame : Type := list term.
 Definition stack : Type := list stack_frame.
 
 (** * Functions *)
@@ -13,10 +13,10 @@ Definition push (sf : stack_frame) (sk : stack) : stack := cons sf sk.
 
 Definition pop (sk : stack) : stack := tl sk.
 
-Definition write_hd (n : nat) (a : tm) (sk : stack) : stack :=
+Definition write_hd (n : nat) (a : term) (sk : stack) : stack :=
   push (replace n a (hd nil sk)) (pop sk).
 
-Definition read_hd (n : nat) (sk : stack) : tm :=
+Definition read_hd (n : nat) (sk : stack) : term :=
   nth n (hd nil sk) tvoid.
 
 Definition resize_hd (n : nat) (sk : stack) : stack :=
