He4/Language/Store.v
@@ -4,16 +4,16 @@ Require Import He4.Lists.List.
 
 (** * Types *)
 
-Definition store : Type := list tm.
+Definition store : Type := list term.
 
 (** * Functions *)
 
-Definition alloc (a : tm) (sr : store) : store :=
+Definition alloc (a : term) (sr : store) : store :=
   app sr (cons a nil).
 
-Definition write (n : nat) (t : tm) (sr : store) : store := replace n t sr.
+Definition write (n : nat) (t : term) (sr : store) : store := replace n t sr.
 
-Definition read (n : nat) (sr : store) : tm := nth n sr tvoid.
+Definition read (n : nat) (sr : store) : term := nth n sr tvoid.
 
 (** TODO: Lemmas *)
 
